imp_system/mem/MemTactics.v
@@ -16,10 +16,12 @@ Section mem.
   Context (ps pt : bool).
   Context (st_src st_tgt : state).
 
+  Context (sp: sp_type).
+
   Lemma wsim_mem_alloc (sz : Z) k_s k_t E1 E2 r g img_t msk_t scp_t msk_m :
     alist_find (Some MemHdr.alloc) fl_t =
       Some (SB.sandbox_body
-        (SModTr.trans_ktree sp_none
+        (SModTr.trans_ktree sp
           (true, msk_m, MemA.scopes, (Some (to_fspec MemSpec.alloc), fbody_trivial)))) →
     (msk_t MemHdr.alloc : bool) →
     (0 <= 8 * sz < modulus_64)%Z →
@@ -44,7 +46,7 @@ Section mem.
   Lemma wsim_mem_store b ofs v v' k_s k_t E1 E2 r g img_t msk_t scp_t msk_m :
     alist_find (Some MemHdr.store) fl_t =
       Some (SB.sandbox_body
-        (SModTr.trans_ktree sp_none
+        (SModTr.trans_ktree sp
           (true, msk_m, MemA.scopes, (Some (to_fspec MemSpec.store), fbody_trivial)))) →
     (msk_t MemHdr.store : bool) →
     (b, ofs) ↦ v' -∗
@@ -67,7 +69,7 @@ Section mem.
   Lemma wsim_mem_load b ofs q v k_s k_t E1 E2 r g img_t msk_t scp_t msk_m :
     alist_find (Some MemHdr.load) fl_t =
       Some (SB.sandbox_body
-        (SModTr.trans_ktree sp_none
+        (SModTr.trans_ktree sp
           (true, msk_m, MemA.scopes, (Some (to_fspec MemSpec.load), fbody_trivial)))) →
     (msk_t MemHdr.load : bool) →
     (b, ofs) ↦{q} v -∗
@@ -90,7 +92,7 @@ Section mem.
   Lemma wsim_mem_cas b ofs v v_old v_new succ E k_s k_t E1 E2 r g img_t msk_t scp_t msk_m :
     alist_find (Some MemHdr.cas) fl_t =
       Some (SB.sandbox_body
-        (SModTr.trans_ktree sp_none
+        (SModTr.trans_ktree sp
           (true, msk_m, MemA.scopes, (Some (to_fspec MemSpec.cas), fbody_trivial)))) →
     (msk_t MemHdr.cas : bool) →
     MemSpec.compare_val v v_old = Vint succ →
@@ -120,7 +122,7 @@ Section mem.
   Lemma wsim_mem_cmp v1 v2 succ E k_s k_t E1 E2 r g img_t msk_t scp_t msk_m :
     alist_find (Some MemHdr.cmp) fl_t =
       Some (SB.sandbox_body
-        (SModTr.trans_ktree sp_none
+        (SModTr.trans_ktree sp
           (true, msk_m, MemA.scopes, (Some (to_fspec MemSpec.cmp), fbody_trivial)))) →
     (msk_t MemHdr.cmp : bool) →
     MemSpec.compare_val v1 v2 = Vint succ →
